Launchbury/Denotational-Related.thy
@@ -46,7 +46,7 @@ next
   have "fdom \<rho> = fdom \<sigma>" using Let(3) by auto
 
   have "\<lbrace>asToHeap as\<rbrace>\<rho> f\<triangleleft>\<triangleright> \<N>\<lbrace>asToHeap as\<rbrace>\<sigma>"
-  proof (rule parallel_UHSem_ind_different_ESem[OF fmap_similar_adm])
+  proof (rule parallel_HSem_ind_different_ESem[OF fmap_similar_adm])
     case goal1 show ?case by (simp add: `fdom \<rho> = fdom \<sigma>`)
   next
     case (goal2 \<rho>' \<sigma>')
@@ -66,7 +66,7 @@ next
 qed
 
 theorem heaps_similar: "\<lbrace>\<Gamma>\<rbrace> f\<triangleleft>\<triangleright> \<N>\<lbrace>\<Gamma>\<rbrace>"
-  by (rule parallel_UHSem_ind_different_ESem[OF fmap_similar_adm])
+  by (rule parallel_HSem_ind_different_ESem[OF fmap_similar_adm])
      (auto simp add: lookupHeapToEnv denotational_semantics_similar)
 
 end
